protobuf-shim/proofs/fstar/extraction/Protobuf.Enum_or_unknown.fsti
@@ -3,4 +3,22 @@ module Protobuf.Enum_or_unknown
 open Core
 open FStar.Mul
 
-type t_EnumOrUnknown (v_E: Type0) = { f_phantom:Core.Marker.t_PhantomData v_E }
+let _ =
+  (* This module has implicit dependencies, here we make them explicit. *)
+  (* The implicit dependencies arise from typeclasses instances. *)
+  let open Protobuf.Enums in
+  ()
+
+type t_EnumOrUnknown (v_E: Type0) = {
+  f_value:i32;
+  f_phantom:Core.Marker.t_PhantomData v_E
+}
+
+val impl__enum_value (#v_E: Type0) {| i1: Protobuf.Enums.t_Enum v_E |} (self: t_EnumOrUnknown v_E)
+    : Prims.Pure (Core.Result.t_Result v_E i32) Prims.l_True (fun _ -> Prims.l_True)
+
+val impl__enum_value_or_default
+      (#v_E: Type0)
+      {| i2: Protobuf.Enums.t_Enum v_E |}
+      (self: t_EnumOrUnknown v_E)
+    : Prims.Pure v_E Prims.l_True (fun _ -> Prims.l_True)
