protobuf-shim/proofs/fstar/extraction/Protobuf.Enum_or_unknown.fst
@@ -1,0 +1,31 @@
+module Protobuf.Enum_or_unknown
+#set-options "--fuel 0 --ifuel 1 --z3rlimit 15"
+open Core
+open FStar.Mul
+
+let _ =
+  (* This module has implicit dependencies, here we make them explicit. *)
+  (* The implicit dependencies arise from typeclasses instances. *)
+  let open Protobuf.Enums in
+  ()
+
+let impl__enum_value
+      (#v_E: Type0)
+      (#[FStar.Tactics.Typeclasses.tcresolve ()] i1: Protobuf.Enums.t_Enum v_E)
+      (self: t_EnumOrUnknown v_E)
+     =
+  Core.Option.impl__ok_or #v_E
+    #i32
+    (Protobuf.Enums.f_from_i32 #v_E #FStar.Tactics.Typeclasses.solve self.f_value
+      <:
+      Core.Option.t_Option v_E)
+    self.f_value
+
+let impl__enum_value_or_default
+      (#v_E: Type0)
+      (#[FStar.Tactics.Typeclasses.tcresolve ()] i2: Protobuf.Enums.t_Enum v_E)
+      (self: t_EnumOrUnknown v_E)
+     =
+  Core.Result.impl__unwrap_or_default #v_E
+    #i32
+    (impl__enum_value #v_E self <: Core.Result.t_Result v_E i32)
